src/Init/Data/Iterators/Lemmas/Consumers/Monadic/Loop.lean
@@ -467,27 +467,33 @@ theorem IterM.drain_eq_map_toArray {α β : Type w} {m : Type w → Type w'} [It
     it.drain = (fun _ => .unit) <$> it.toList := by
   simp [IterM.drain_eq_map_toList]
 
-theorem IterM.count_eq_fold {α β : Type w} {m : Type w → Type w'} [Iterator α m β]
+theorem IterM.length_eq_fold {α β : Type w} {m : Type w → Type w'} [Iterator α m β]
     [Finite α m] [Monad m] [LawfulMonad m] [IteratorLoop α m m]
     {it : IterM (α := α) m β} :
-    it.count = it.fold (init := .up 0) (fun acc _ => .up <| acc.down + 1) :=
+    it.length = it.fold (init := .up 0) (fun acc _ => .up <| acc.down + 1) :=
   (rfl)
 
-theorem IterM.count_eq_forIn {α β : Type w} {m : Type w → Type w'} [Iterator α m β]
+@[deprecated IterM.length_eq_fold (since := "2026-01-28")]
+def IterM.count_eq_fold := @IterM.length_eq_fold
+
+theorem IterM.length_eq_forIn {α β : Type w} {m : Type w → Type w'} [Iterator α m β]
     [Finite α m] [Monad m] [LawfulMonad m] [IteratorLoop α m m]
     {it : IterM (α := α) m β} :
-    it.count = ForIn.forIn it (.up 0) (fun _ acc => return .yield (.up (acc.down + 1))) :=
+    it.length = ForIn.forIn it (.up 0) (fun _ acc => return .yield (.up (acc.down + 1))) :=
   (rfl)
 
-theorem IterM.count_eq_match_step {α β : Type w} {m : Type w → Type w'} [Iterator α m β]
+@[deprecated IterM.length_eq_forIn (since := "2026-01-28")]
+def IterM.count_eq_forIn := @IterM.length_eq_forIn
+
+theorem IterM.length_eq_match_step {α β : Type w} {m : Type w → Type w'} [Iterator α m β]
     [Finite α m] [Monad m] [LawfulMonad m] [IteratorLoop α m m] [LawfulIteratorLoop α m m]
     {it : IterM (α := α) m β} :
-    it.count = (do
+    it.length = (do
       match (← it.step).inflate.val with
-      | .yield it' _ => return .up ((← it'.count).down + 1)
-      | .skip it' => return .up (← it'.count).down
+      | .yield it' _ => return .up ((← it'.length).down + 1)
+      | .skip it' => return .up (← it'.length).down
       | .done => return .up 0) := by
-  simp only [count_eq_fold]
+  simp only [length_eq_fold]
   have (acc : Nat) (it' : IterM (α := α) m β) :
       it'.fold (init := ULift.up acc) (fun acc _ => .up (acc.down + 1)) =
         (ULift.up <| ·.down + acc) <$>
@@ -503,33 +509,45 @@ theorem IterM.count_eq_match_step {α β : Type w} {m : Type w → Type w'} [Ite
   · simp
   · simp
 
+@[deprecated IterM.length_eq_match_step (since := "2026-01-28")]
+def IterM.count_eq_match_step := @IterM.length_eq_match_step
+
 @[simp]
-theorem IterM.up_size_toArray_eq_count {α β : Type w} [Iterator α m β] [Finite α m]
+theorem IterM.up_size_toArray_eq_length {α β : Type w} [Iterator α m β] [Finite α m]
     [Monad m] [LawfulMonad m]
     [IteratorLoop α m m] [LawfulIteratorLoop α m m]
     {it : IterM (α := α) m β} :
-    (.up <| ·.size) <$> it.toArray = it.count := by
-  rw [toArray_eq_fold, count_eq_fold, ← fold_hom]
+    (.up <| ·.size) <$> it.toArray = it.length := by
+  rw [toArray_eq_fold, length_eq_fold, ← fold_hom]
   · simp only [List.size_toArray, List.length_nil]; rfl
   · simp
 
+@[deprecated IterM.up_size_toArray_eq_length (since := "2026-01-28")]
+def IterM.up_size_toArray_eq_count := @IterM.up_size_toArray_eq_length
+
 @[simp]
-theorem IterM.up_length_toList_eq_count {α β : Type w} [Iterator α m β] [Finite α m]
+theorem IterM.up_length_toList_eq_length {α β : Type w} [Iterator α m β] [Finite α m]
     [Monad m] [LawfulMonad m]
     [IteratorLoop α m m] [LawfulIteratorLoop α m m]
     {it : IterM (α := α) m β} :
-    (.up <| ·.length) <$> it.toList = it.count := by
-  rw [toList_eq_fold, count_eq_fold, ← fold_hom]
+    (.up <| ·.length) <$> it.toList = it.length := by
+  rw [toList_eq_fold, length_eq_fold, ← fold_hom]
   · simp only [List.length_nil]; rfl
   · simp
 
+@[deprecated IterM.up_length_toList_eq_length (since := "2026-01-28")]
+def IterM.up_length_toList_eq_count := @IterM.up_length_toList_eq_length
+
 @[simp]
-theorem IterM.up_length_toListRev_eq_count {α β : Type w} [Iterator α m β] [Finite α m]
+theorem IterM.up_length_toListRev_eq_length {α β : Type w} [Iterator α m β] [Finite α m]
     [Monad m] [LawfulMonad m]
     [IteratorLoop α m m] [LawfulIteratorLoop α m m]
     {it : IterM (α := α) m β} :
-    (.up <| ·.length) <$> it.toListRev = it.count := by
-  simp only [toListRev_eq, Functor.map_map, List.length_reverse, up_length_toList_eq_count]
+    (.up <| ·.length) <$> it.toListRev = it.length := by
+  simp only [toListRev_eq, Functor.map_map, List.length_reverse, up_length_toList_eq_length]
+
+@[deprecated IterM.up_length_toListRev_eq_length (since := "2026-01-28")]
+def IterM.up_length_toListRev_eq_count := @IterM.up_length_toListRev_eq_length
 
 theorem IterM.anyM_eq_forIn {α β : Type w} {m : Type w → Type w'} [Iterator α m β]
     [Finite α m] [Monad m] [LawfulMonad m] [IteratorLoop α m m] [LawfulIteratorLoop α m m]
