src/Std/Data/Iterators/Lemmas/Producers/Range.lean
@@ -39,19 +39,26 @@ theorem Rcc.toArray_iter_eq_toArray [LE α] [DecidableLE α] [UpwardEnumerable �
  rfl
 
 @[simp]
+theorem Rcc.length_iter [LE α] [DecidableLE α] [UpwardEnumerable α]
+    [LawfulUpwardEnumerableLE α] [Rxc.IsAlwaysFinite α] [LawfulUpwardEnumerable α]
+    [Rxc.HasSize α] [Rxc.LawfulHasSize α] {r : Rcc α} :
+    r.iter.length = r.size := by
+  rw [← size_toArray, ← toArray_iter, Iter.size_toArray_eq_length]
+
+@[deprecated Rcc.length_iter (since := "2026-01-28")]
 theorem Rcc.count_iter [LE α] [DecidableLE α] [UpwardEnumerable α]
     [LawfulUpwardEnumerableLE α] [Rxc.IsAlwaysFinite α] [LawfulUpwardEnumerable α]
     [Rxc.HasSize α] [Rxc.LawfulHasSize α] {r : Rcc α} :
-    r.iter.count = r.size := by
-  rw [← size_toArray, ← toArray_iter, Iter.size_toArray_eq_count]
+    r.iter.length = r.size :=
+  length_iter
 
-@[deprecated Rcc.count_iter (since := "2025-11-13")]
+@[deprecated Rcc.length_iter (since := "2025-11-13")]
 theorem Rcc.count_iter_eq_size [LE α] [DecidableLE α] [UpwardEnumerable α]
     [LawfulUpwardEnumerableLE α] [Rxc.IsAlwaysFinite α] [LawfulUpwardEnumerable α]
     [Rxc.HasSize α] [Rxc.LawfulHasSize α]
     {r : Rcc α} :
-    r.iter.count = r.size :=
-  count_iter
+    r.iter.length = r.size :=
+  length_iter
 
 @[simp]
 theorem Rco.toList_iter [LT α] [DecidableLT α] [UpwardEnumerable α]
@@ -78,20 +85,28 @@ theorem Rco.toArray_iter_eq_toArray [LT α] [DecidableLT α] [UpwardEnumerable �
  rfl
 
 @[simp]
+theorem Rco.length_iter [LT α] [DecidableLT α] [UpwardEnumerable α]
+    [LawfulUpwardEnumerableLT α] [Rxo.IsAlwaysFinite α] [LawfulUpwardEnumerable α]
+    [Rxo.HasSize α] [Rxo.LawfulHasSize α]
+    {r : Rco α} :
+    r.iter.length = r.size := by
+  rw [← size_toArray, ← toArray_iter, Iter.size_toArray_eq_length]
+
+@[deprecated Rco.length_iter (since := "2026-01-28")]
 theorem Rco.count_iter [LT α] [DecidableLT α] [UpwardEnumerable α]
     [LawfulUpwardEnumerableLT α] [Rxo.IsAlwaysFinite α] [LawfulUpwardEnumerable α]
     [Rxo.HasSize α] [Rxo.LawfulHasSize α]
     {r : Rco α} :
-    r.iter.count = r.size := by
-  rw [← size_toArray, ← toArray_iter, Iter.size_toArray_eq_count]
+    r.iter.length = r.size := by
+  rw [← size_toArray, ← toArray_iter, Iter.size_toArray_eq_length]
 
-@[deprecated Rco.count_iter (since := "2025-11-13")]
+@[deprecated Rco.length_iter (since := "2025-11-13")]
 theorem Rco.count_iter_eq_size [LT α] [DecidableLT α] [UpwardEnumerable α]
     [LawfulUpwardEnumerableLT α] [Rxo.IsAlwaysFinite α] [LawfulUpwardEnumerable α]
     [Rxo.HasSize α] [Rxo.LawfulHasSize α]
     {r : Rco α} :
-    r.iter.count = r.size := by
-  rw [← size_toArray, ← toArray_iter, Iter.size_toArray_eq_count]
+    r.iter.length = r.size := by
+  rw [← size_toArray, ← toArray_iter, Iter.size_toArray_eq_length]
 
 @[simp]
 theorem Rci.toList_iter [UpwardEnumerable α]
@@ -118,20 +133,28 @@ theorem Rci.toArray_iter_eq_toArray [UpwardEnumerable α]
  rfl
 
 @[simp]
+theorem Rci.length_iter [UpwardEnumerable α]
+    [Rxi.IsAlwaysFinite α] [LawfulUpwardEnumerable α]
+    [Rxi.HasSize α] [Rxi.LawfulHasSize α]
+    {r : Rci α} :
+    r.iter.length = r.size := by
+  rw [← size_toArray, ← toArray_iter_eq_toArray, Iter.size_toArray_eq_length]
+
+@[deprecated Rci.length_iter (since := "2026-01-28")]
 theorem Rci.count_iter [UpwardEnumerable α]
     [Rxi.IsAlwaysFinite α] [LawfulUpwardEnumerable α]
     [Rxi.HasSize α] [Rxi.LawfulHasSize α]
     {r : Rci α} :
-    r.iter.count = r.size := by
-  rw [← size_toArray, ← toArray_iter_eq_toArray, Iter.size_toArray_eq_count]
+    r.iter.length = r.size := by
+  rw [← size_toArray, ← toArray_iter_eq_toArray, Iter.size_toArray_eq_length]
 
-@[deprecated Rci.count_iter (since := "2025-11-13")]
+@[deprecated Rci.length_iter (since := "2025-11-13")]
 theorem Rci.count_iter_eq_size [UpwardEnumerable α]
     [Rxi.IsAlwaysFinite α] [LawfulUpwardEnumerable α]
     [Rxi.HasSize α] [Rxi.LawfulHasSize α]
     {r : Rci α} :
-    r.iter.count = r.size := by
-  rw [← size_toArray, ← toArray_iter_eq_toArray, Iter.size_toArray_eq_count]
+    r.iter.length = r.size := by
+  rw [← size_toArray, ← toArray_iter_eq_toArray, Iter.size_toArray_eq_length]
 
 @[simp]
 theorem Roc.toList_iter [LE α] [DecidableLE α] [UpwardEnumerable α]
@@ -158,20 +181,28 @@ theorem Roc.toArray_iter_eq_toArray [LE α] [DecidableLE α] [UpwardEnumerable �
  rfl
 
 @[simp]
+theorem Roc.length_iter [LE α] [DecidableLE α] [UpwardEnumerable α]
+    [LawfulUpwardEnumerableLE α] [Rxc.IsAlwaysFinite α] [LawfulUpwardEnumerable α]
+    [Rxc.HasSize α] [Rxc.LawfulHasSize α]
+    {r : Roc α} :
+    r.iter.length = r.size := by
+  rw [← size_toArray, ← toArray_iter_eq_toArray, Iter.size_toArray_eq_length]
+
+@[deprecated Roc.length_iter (since := "2026-01-28")]
 theorem Roc.count_iter [LE α] [DecidableLE α] [UpwardEnumerable α]
     [LawfulUpwardEnumerableLE α] [Rxc.IsAlwaysFinite α] [LawfulUpwardEnumerable α]
     [Rxc.HasSize α] [Rxc.LawfulHasSize α]
     {r : Roc α} :
-    r.iter.count = r.size := by
-  rw [← size_toArray, ← toArray_iter_eq_toArray, Iter.size_toArray_eq_count]
+    r.iter.length = r.size := by
+  rw [← size_toArray, ← toArray_iter_eq_toArray, Iter.size_toArray_eq_length]
 
-@[deprecated Roc.count_iter (since := "2025-11-13")]
+@[deprecated Roc.length_iter (since := "2025-11-13")]
 theorem Roc.count_iter_eq_size [LE α] [DecidableLE α] [UpwardEnumerable α]
     [LawfulUpwardEnumerableLE α] [Rxc.IsAlwaysFinite α] [LawfulUpwardEnumerable α]
     [Rxc.HasSize α] [Rxc.LawfulHasSize α]
     {r : Roc α} :
-    r.iter.count = r.size := by
-  rw [← size_toArray, ← toArray_iter_eq_toArray, Iter.size_toArray_eq_count]
+    r.iter.length = r.size := by
+  rw [← size_toArray, ← toArray_iter_eq_toArray, Iter.size_toArray_eq_length]
 
 @[simp]
 theorem Roo.toList_iter [LT α] [DecidableLT α] [UpwardEnumerable α]
@@ -198,20 +229,28 @@ theorem Roo.toArray_iter_eq_toArray [LT α] [DecidableLT α] [UpwardEnumerable �
  rfl
 
 @[simp]
+theorem Roo.length_iter [LT α] [DecidableLT α] [UpwardEnumerable α]
+    [LawfulUpwardEnumerableLT α] [Rxo.IsAlwaysFinite α] [LawfulUpwardEnumerable α]
+    [Rxo.HasSize α] [Rxo.LawfulHasSize α]
+    {r : Roo α} :
+    r.iter.length = r.size := by
+  rw [← size_toArray, ← toArray_iter_eq_toArray, Iter.size_toArray_eq_length]
+
+@[deprecated Roo.length_iter (since := "2026-01-28")]
 theorem Roo.count_iter [LT α] [DecidableLT α] [UpwardEnumerable α]
     [LawfulUpwardEnumerableLT α] [Rxo.IsAlwaysFinite α] [LawfulUpwardEnumerable α]
     [Rxo.HasSize α] [Rxo.LawfulHasSize α]
     {r : Roo α} :
-    r.iter.count = r.size := by
-  rw [← size_toArray, ← toArray_iter_eq_toArray, Iter.size_toArray_eq_count]
+    r.iter.length = r.size := by
+  rw [← size_toArray, ← toArray_iter_eq_toArray, Iter.size_toArray_eq_length]
 
-@[deprecated Roo.count_iter (since := "2025-11-13")]
+@[deprecated Roo.length_iter (since := "2025-11-13")]
 theorem Roo.count_iter_eq_size [LT α] [DecidableLT α] [UpwardEnumerable α]
     [LawfulUpwardEnumerableLT α] [Rxo.IsAlwaysFinite α] [LawfulUpwardEnumerable α]
     [Rxo.HasSize α] [Rxo.LawfulHasSize α]
     {r : Roo α} :
-    r.iter.count = r.size := by
-  rw [← size_toArray, ← toArray_iter_eq_toArray, Iter.size_toArray_eq_count]
+    r.iter.length = r.size := by
+  rw [← size_toArray, ← toArray_iter_eq_toArray, Iter.size_toArray_eq_length]
 
 @[simp]
 theorem Roi.toList_iter [UpwardEnumerable α]
@@ -238,20 +277,28 @@ theorem Roi.toArray_iter_eq_toArray [UpwardEnumerable α]
  rfl
 
 @[simp]
+theorem Roi.length_iter [UpwardEnumerable α]
+    [Rxi.IsAlwaysFinite α] [LawfulUpwardEnumerable α]
+    [Rxi.HasSize α] [Rxi.LawfulHasSize α]
+    {r : Roi α} :
+    r.iter.length = r.size := by
+  rw [← size_toArray, ← toArray_iter, Iter.size_toArray_eq_length]
+
+@[deprecated Roi.length_iter (since := "2026-01-28")]
 theorem Roi.count_iter [UpwardEnumerable α]
     [Rxi.IsAlwaysFinite α] [LawfulUpwardEnumerable α]
     [Rxi.HasSize α] [Rxi.LawfulHasSize α]
     {r : Roi α} :
-    r.iter.count = r.size := by
-  rw [← size_toArray, ← toArray_iter, Iter.size_toArray_eq_count]
+    r.iter.length = r.size := by
+  rw [← size_toArray, ← toArray_iter, Iter.size_toArray_eq_length]
 
-@[deprecated Roi.count_iter (since := "2025-11-13")]
+@[deprecated Roi.length_iter (since := "2025-11-13")]
 theorem Roi.count_iter_eq_size [UpwardEnumerable α]
     [Rxi.IsAlwaysFinite α] [LawfulUpwardEnumerable α]
     [Rxi.HasSize α] [Rxi.LawfulHasSize α]
     {r : Roi α} :
-    r.iter.count = r.size := by
-  rw [← size_toArray, ← toArray_iter, Iter.size_toArray_eq_count]
+    r.iter.length = r.size := by
+  rw [← size_toArray, ← toArray_iter, Iter.size_toArray_eq_length]
 
 @[simp]
 theorem Ric.toList_iter [Least? α] [LE α] [DecidableLE α] [UpwardEnumerable α]
@@ -278,20 +325,28 @@ theorem Ric.toArray_iter_eq_toArray [Least? α] [LE α] [DecidableLE α] [Upward
  rfl
 
 @[simp]
+theorem Ric.length_iter [Least? α] [LE α] [DecidableLE α] [UpwardEnumerable α]
+    [LawfulUpwardEnumerableLE α] [Rxc.IsAlwaysFinite α] [LawfulUpwardEnumerable α]
+    [Rxc.HasSize α] [Rxc.LawfulHasSize α]
+    {r : Ric α} :
+    r.iter.length = r.size := by
+  rw [← size_toArray, ← toArray_iter, Iter.size_toArray_eq_length]
+
+@[deprecated Ric.length_iter (since := "2026-01-28")]
 theorem Ric.count_iter [Least? α] [LE α] [DecidableLE α] [UpwardEnumerable α]
     [LawfulUpwardEnumerableLE α] [Rxc.IsAlwaysFinite α] [LawfulUpwardEnumerable α]
     [Rxc.HasSize α] [Rxc.LawfulHasSize α]
     {r : Ric α} :
-    r.iter.count = r.size := by
-  rw [← size_toArray, ← toArray_iter, Iter.size_toArray_eq_count]
+    r.iter.length = r.size := by
+  rw [← size_toArray, ← toArray_iter, Iter.size_toArray_eq_length]
 
-@[deprecated Ric.count_iter (since := "2025-11-13")]
+@[deprecated Ric.length_iter (since := "2025-11-13")]
 theorem Ric.count_iter_eq_size [Least? α] [LE α] [DecidableLE α] [UpwardEnumerable α]
     [LawfulUpwardEnumerableLE α] [Rxc.IsAlwaysFinite α] [LawfulUpwardEnumerable α]
     [Rxc.HasSize α] [Rxc.LawfulHasSize α]
     {r : Ric α} :
-    r.iter.count = r.size := by
-  rw [← size_toArray, ← toArray_iter, Iter.size_toArray_eq_count]
+    r.iter.length = r.size := by
+  rw [← size_toArray, ← toArray_iter, Iter.size_toArray_eq_length]
 
 @[simp]
 theorem Rio.toList_iter [Least? α] [LT α] [DecidableLT α] [UpwardEnumerable α]
@@ -318,20 +373,28 @@ theorem Rio.toArray_iter_eq_toArray [Least? α] [LT α] [DecidableLT α] [Upward
  rfl
 
 @[simp]
+theorem Rio.length_iter [Least? α] [LT α] [DecidableLT α] [UpwardEnumerable α]
+    [LawfulUpwardEnumerableLT α] [Rxo.IsAlwaysFinite α] [LawfulUpwardEnumerable α]
+    [Rxo.HasSize α] [Rxo.LawfulHasSize α]
+    {r : Rio α} :
+    r.iter.length = r.size := by
+  rw [← size_toArray, ← toArray_iter, Iter.size_toArray_eq_length]
+
+@[deprecated Rio.length_iter (since := "2026-01-28")]
 theorem Rio.count_iter [Least? α] [LT α] [DecidableLT α] [UpwardEnumerable α]
     [LawfulUpwardEnumerableLT α] [Rxo.IsAlwaysFinite α] [LawfulUpwardEnumerable α]
     [Rxo.HasSize α] [Rxo.LawfulHasSize α]
     {r : Rio α} :
-    r.iter.count = r.size := by
-  rw [← size_toArray, ← toArray_iter, Iter.size_toArray_eq_count]
+    r.iter.length = r.size := by
+  rw [← size_toArray, ← toArray_iter, Iter.size_toArray_eq_length]
 
-@[deprecated Rio.count_iter (since := "2025-11-13")]
+@[deprecated Rio.length_iter (since := "2025-11-13")]
 theorem Rio.count_iter_eq_size [Least? α] [LT α] [DecidableLT α] [UpwardEnumerable α]
     [LawfulUpwardEnumerableLT α] [Rxo.IsAlwaysFinite α] [LawfulUpwardEnumerable α]
     [Rxo.HasSize α] [Rxo.LawfulHasSize α]
     {r : Rio α} :
-    r.iter.count = r.size := by
-  rw [← size_toArray, ← toArray_iter, Iter.size_toArray_eq_count]
+    r.iter.length = r.size := by
+  rw [← size_toArray, ← toArray_iter, Iter.size_toArray_eq_length]
 
 @[simp]
 theorem Rii.toList_iter [Least? α] [UpwardEnumerable α]
@@ -358,19 +421,27 @@ theorem Rii.toArray_iter_eq_toArray [Least? α] [UpwardEnumerable α]
  rfl
 
 @[simp]
+theorem Rii.length_iter [Least? α] [UpwardEnumerable α]
+    [Rxi.IsAlwaysFinite α] [LawfulUpwardEnumerable α]
+    [Rxi.HasSize α] [Rxi.LawfulHasSize α]
+    {r : Rii α} :
+    r.iter.length = r.size := by
+  rw [← size_toArray, ← toArray_iter, Iter.size_toArray_eq_length]
+
+@[deprecated Rii.length_iter (since := "2026-01-28")]
 theorem Rii.count_iter [Least? α] [UpwardEnumerable α]
     [Rxi.IsAlwaysFinite α] [LawfulUpwardEnumerable α]
     [Rxi.HasSize α] [Rxi.LawfulHasSize α]
     {r : Rii α} :
-    r.iter.count = r.size := by
-  rw [← size_toArray, ← toArray_iter, Iter.size_toArray_eq_count]
+    r.iter.length = r.size := by
+  rw [← size_toArray, ← toArray_iter, Iter.size_toArray_eq_length]
 
-@[deprecated Rii.count_iter (since := "2025-11-13")]
+@[deprecated Rii.length_iter (since := "2025-11-13")]
 theorem Rii.count_iter_eq_size [Least? α] [UpwardEnumerable α]
     [Rxi.IsAlwaysFinite α] [LawfulUpwardEnumerable α]
     [Rxi.HasSize α] [Rxi.LawfulHasSize α]
     {r : Rii α} :
-    r.iter.count = r.size := by
-  rw [← size_toArray, ← toArray_iter, Iter.size_toArray_eq_count]
+    r.iter.length = r.size := by
+  rw [← size_toArray, ← toArray_iter, Iter.size_toArray_eq_length]
 
 end Std
